working bitwiseu16op

SP1Operations/BitWiseU16Operation.lean
@@ -7,49 +7,45 @@ import LeanRV32D.RiscvRegs
 open LeanRV32D.Functions
 
 structure BitwiseU16Operation where
+  a_low_bytes : U16toU8Operation
   b_low_bytes : U16toU8Operation
-  c_low_bytes : U16toU8Operation
   bitwise_operation : BitwiseOperation
 
 namespace BitwiseU16Operation
 
-def constraint
+def constraintList
+  (a : Word BabyBear)
   (b : Word BabyBear)
-  (cc : Word BabyBear)
   (cols : BitwiseU16Operation)
   (opcode : BabyBear)
   (is_real : BabyBear)
-  : Word BabyBear × List SP1Constraint :=
+  : Word BabyBear × SP1ConstraintList :=
   let E0 : BabyBear := is_real - 1
   let E2 : BabyBear := is_real * E0
 
   let ⟨V0, CS0⟩ := U16ToU8OperationUnsafe.constraints
+    #v[a[0], a[1]]
+    { low_bytes :=
+        #v[cols.a_low_bytes.low_bytes[0]
+        , cols.a_low_bytes.low_bytes[1]
+        ]
+    }
+  let E4 : BabyBear := V0[0]
+  let E5 : BabyBear := V0[1]
+  let E6 : BabyBear := V0[2]
+  let E7 : BabyBear := V0[3]
+
+  let ⟨V1, CS1⟩ := U16ToU8OperationUnsafe.constraints
     #v[b[0], b[1]]
     { low_bytes :=
         #v[cols.b_low_bytes.low_bytes[0]
         , cols.b_low_bytes.low_bytes[1]
         ]
     }
-  -- We will have our own syntax to pattern match
-  -- Vector BabyBear WORD_BYTE_SIZE
-  let E4 : BabyBear := V0[0]
-  let E5 : BabyBear := V0[1]
-  let E6 : BabyBear := V0[1]
-  let E7 : BabyBear := V0[1]
-
-  let ⟨V1, CS1⟩ := U16ToU8OperationUnsafe.constraints
-    #v[cc[0], cc[1]]
-    { low_bytes :=
-        #v[cols.c_low_bytes.low_bytes[0]
-        , cols.c_low_bytes.low_bytes[1]
-        ]
-    }
-  -- We will have our own syntax to pattern match
-  -- Vector BabyBear WORD_BYTE_SIZE
-  let E8 : BabyBear := V0[0]
-  let E9 : BabyBear := V0[1]
-  let E10 : BabyBear := V0[1]
-  let E11 : BabyBear := V0[1]
+  let E8 : BabyBear := V1[0]
+  let E9 : BabyBear := V1[1]
+  let E10 : BabyBear := V1[2]
+  let E11 : BabyBear := V1[3]
 
   let E12 : BabyBear := cols.bitwise_operation.result[1] * 256
   let E14 : BabyBear := E8 + E12
@@ -69,5 +65,46 @@ def constraint
           ] }
       opcode
       is_real)⟩
+
+def spec
+    (a : Word BabyBear)
+    (b : Word BabyBear)
+    (cols : BitwiseU16Operation)
+    (opcode : BabyBear)
+    (is_real : BabyBear) : Prop :=
+  -- let cr := cols.bitwise_operation.result
+  is_real ≠ 0 →
+    BitwiseOperation.spec
+      (#v[cols.a_low_bytes.low_bytes[0], (a[0] - cols.a_low_bytes.low_bytes[0]) * 2005401601,
+          cols.a_low_bytes.low_bytes[1], (a[1] - cols.a_low_bytes.low_bytes[1]) * 2005401601])
+      (#v[cols.b_low_bytes.low_bytes[0], (b[0] - cols.b_low_bytes.low_bytes[0]) * 2005401601,
+          cols.b_low_bytes.low_bytes[1], (b[1] - cols.b_low_bytes.low_bytes[1]) * 2005401601])
+      cols.bitwise_operation
+      opcode
+
+lemma constraintList_imp_spec
+    (a : Word BabyBear)
+    (b : Word BabyBear)
+    (cols : BitwiseU16Operation)
+    (opcode : BabyBear)
+    (is_real : BabyBear) :
+    (constraintList a b cols opcode is_real).2.allHold → (spec a b cols opcode is_real) := by
+  rw [constraintList, spec]
+  intro h h_is_real
+  simp only [WORD_SIZE, BabyBearPrime, Fin.isValue]
+  refine BitwiseOperation.constraints_imp_spec
+    (#v[cols.a_low_bytes.low_bytes[0], (a[0] - cols.a_low_bytes.low_bytes[0]) * 2005401601,
+        cols.a_low_bytes.low_bytes[1], (a[1] - cols.a_low_bytes.low_bytes[1]) * 2005401601])
+    (#v[cols.b_low_bytes.low_bytes[0], (b[0] - cols.b_low_bytes.low_bytes[0]) * 2005401601,
+        cols.b_low_bytes.low_bytes[1], (b[1] - cols.b_low_bytes.low_bytes[1]) * 2005401601])
+    cols.bitwise_operation
+    opcode is_real h_is_real ?_
+  simp [] at h
+
+  -- This is hacky, need some extensionality thing instead
+  convert h.2 using 1
+
+-- TODO: pull forward lemmas about `BitWiseOperation.spec` to this `spec`
+
 
 end BitwiseU16Operation
